# verify_solution

Tasks where a provided skill's *name* is reproduced verbatim

Frequency: 1

Lemma:
```isabelle
lemma verify_solution:
  fixes x y :: real
  assumes "x = 9 - 2 * y" and "y = 3 * x + 1"
  shows "x = 1 \<and> y = 4"
proof -
  from assms(2) have "y = 3 * x + 1" by simp
  from assms(1) have "x = 9 - 2 * y" by simp
  then have "y = 3 * (9 - 2 * y) + 1" by (simp only: assms(2))
  then have "y = 27 - 6 * y + 1" by (simp add: algebra_simps)
  then have "y = 28 - 6 * y" by simp
  then have "y + 6 * y = 28" by (simp add: add.commute)
  then have "7 * y = 28" by (simp add: algebra_simps)
  then have "y = 4" by (simp add: mult.commute)
  with assms(1) have "x = 9 - 2 * 4" by (simp only: assms(1))
  then have "x = 1" by simp
  then show "x = 1 \<and> y = 4" by (metis \<open>y = 4\<close>)
qed
```


## Usage 1 of 1:
### Problem:
Task name: `mathd_algebra_44.json`

At which point do the lines $s=9-2t$ and $t=3s+1$ intersect? Give your answer as an ordered pair in the form $(s, t).$ Show that it is (1,4).
### Informal Proof:
We can substitute the second equation into the first equation to get  $$s=9-2(3s+1)=9-6s-2.$$Moving the variable terms to the left-hand side and the constants to the right-hand side, we find $$s+6s=7.$$This gives  $s=1$ which we may plug into either equation to get $t$. For example, $$t=3(1)+1=4.$$So the lines intersect at the point $(1,4)$.
### Solution:
```isabelle
theorem mathd_algebra_44:
  fixes s t :: real
  assumes "s = 9 - 2 * t"
    and "t = 3 * s + 1" 
  shows "s = 1 \<and> t = 4"
```
AI Generated completion (lemma lines higlighted):
<think>
Okay, let's see. The user wants me to provide a formal proof in Isabelle for the problem where two lines intersect at (1,4). The problem gives the equations s = 9 - 2t and t = 3s + 1. The formal statement is already provided, so I need to structure the proof step by step, using the given lemmas and following the structure from the examples.

First, I should recall the useful skills provided. For example, the solve_linear_substitution lemma was used in previous problems. Maybe I can use that here. But looking at the problem, it's a system of two equations with two variables, so substitution is the way to go.

The informal proof steps are substitution, simplifying, solving for s, then t, and verifying. The formal proof should mirror these steps. Let me think about each step.

In the first step of the informal proof, they substitute t from the second equation into the first. So in Isabelle, I can use the second assumption to replace t in the first equation. The lemma verify_solution from the examples might be helpful here, but maybe I can create a similar structure. %%%%%%%%%%%%%%%%%%%%%%%%%%%%%%%%%%%%%%%%%%%%%%%%%%

Let me check the given lemmas. The solve_linear_substitution lemma shows substitution, but here we have a system where each variable is expressed in terms of the other. So substituting t from the second equation into the first gives s = 9 - 2*(3s + 1). Then simplifying that equation to solve for s.

In Isabelle, I can use the 'also' and 'finally' methods for substitution. For example, from the second assumption, we have t = 3s +1. Substitute that into the first equation's right-hand side. Then simplify.

After substitution, the equation becomes s = 9 - 2*(3s +1). Simplify that to s = 9 -6s -2 → s = 7 -6s. Then bringing terms together: s +6s =7 →7s=7 →s=1. Then substitute back to find t.

So in the proof steps, I need to:

1. Substitute t from the second equation into the first.
2. Simplify the resulting equation to solve for s.
3. Once s is found, substitute back to find t.
4. Verify that these values satisfy both equations.

In Isabelle, using the 'also' and 'finally' notation can help. Also, using algebra_simps for simplification steps. The lemma cancle_div might not be needed here, but maybe the solve_linear_substitution can be applied.

Wait, the given lemma solve_linear_substitution is for variables x and y with equations x = a - b*y and y = c*x +d, leading to x = a -b*(c*x +d). That's exactly the substitution step here. So in this problem, s = 9 -2t and t =3s +1. So substituting t into the first equation gives s =9 -2*(3s +1). Which is exactly the case of the lemma. So maybe I can use that lemma here.

But the lemma is for general a, b, c, d, x, y. So in this case, a=9, b=2, c=3, d=1, x=s, y=t. So applying the lemma would give s =9 -2*(3s +1). Then proceed to solve that equation.

So the first step would be to use the lemma to substitute, then solve for s.

But the user's previous example used the solve_linear_substitution lemma. So maybe I can use that here.

Alternatively, I can write the substitution manually, using the assumptions. Let me check the code.

The theorem's proof starts with:

proof -
  from assms(2) have t_eq: "t = 3*s + 1" by simp
  from assms(1) have "s = 9 - 2*t" by simp
  then have "s = 9 - 2*(3*s + 1)" by (metis t_eq)
  thus ?thesis by ... ?

Wait, but the next steps would be to solve that equation. Let's see.

So after substitution, the equation is s = 9 - 2*(3s +1). Simplify that:

s = 9 -6s -2 → s =7 -6s → 7s =7 →s=1.

Then substitute back into t =3s +1 → t=3*1 +1=4.

So in Isabelle, I can do:

Then have "s = 9 - 2*(3*s + 1)" by (simp only: t_eq)
Then simplify that equation. Let's see:

s = 9 - 6s -2 → s =7 -6s. So:

have "s = 7 - 6*s" by (simp add: algebra_simps)

Then, adding 6s to both sides:

s +6s =7 →7s=7 →s=1.

So:

then have "s + 6*s = 7" by (simp add: add.commute)
then have "7*s =7" by (simp add: algebra_simps)
then have "s=1" by (simp add: mult.commute)

Once s is found, substitute back into the second equation to get t.

Then, using t=3s+1 with s=1:

have "t = 3*1 +1" by (simp only: assms(2))
then have "t=4" by simp.

Finally, show that s=1 and t=4.

But in the formal statement, the conclusion is "s =1 ∧ t=4".

So putting all these steps together with proper justifications.

I need to make sure that each step is justified by the assumptions or previous steps. Also, using the lemmas if possible. The user mentioned that creating reusable lemmas is encouraged. However, in this problem, the steps are straightforward substitution and solving linear equations, which might not require a new lemma, but perhaps using the existing ones.

Alternatively, maybe the lemma solve_linear_substitution can be used here. Let me check the lemma again:

lemma solve_linear_substitution:
  fixes a b c d x y :: real
  assumes "x = a - b * y" and "y = c * x + d"
  shows "x = (a - b * (c * x + d))" 

So in our case, x is s, y is t, a=9, b=2, c=3, d=1. So applying this lemma would give s=9 -2*(3s +1), which is the substitution step. Then proceed to solve for s.

So maybe in the proof, first apply this lemma, then solve the resulting equation.

But the user's previous example used this lemma, and then solved the equation step by step.

So the proof could be structured as:

proof -
  have "s = 9 - 2*(3*s + 1)" using solve_linear_substitution with the given assumptions.
  Then simplify to find s=1, then find t=4.

But in Isabelle, the lemma needs to be applied correctly. Let me check the code.

Alternatively, using the 'also' and 'finally' approach.

Another approach is to use the given lemma verify_solution, which was used in the mathd_numbertheory_284 problem. However, that problem had different equations. But the structure is similar. %%%%%%%%%%%%%%%%%%%%%%%%%%%%%%%%%%%%%%%%%%%%%%%%%%

In any case, the key steps are substitution, solving for s, then t, and verifying.

So putting this all together, the Isabelle proof would look like:

proof -
  from assms(2) have t_eq: "t = 3*s + 1" by simp
  from assms(1) have s_eq: "s = 9 - 2*t" by simp
  then have "s = 9 - 2*(3*s + 1)" by (metis t_eq)
  then have "s = 7 - 6*s" by (simp add: algebra_simps)
  then have "s + 6*s = 7" by (simp add: add.commute)
  then have "7*s = 7" by (simp add: algebra_simps)
  then have "s = 1" by (simp add: mult.commute)
  with t_eq have "t = 3*1 + 1" by simp
  then have "t = 4" by simp
  then show "s = 1 ∧ t = 4" by (metis s=1 t=4)
qed

But I need to make sure each step is properly justified with the correct rules. Also, the 'metis' call might be needed to combine the conclusions.

Alternatively, using 'then' and 'also' steps.

Another thing to note is that in the given lemma verify_solution, they used sledgehammer for some steps, but here, the steps are straightforward and can be handled with algebra_simps and simplification. %%%%%%%%%%%%%%%%%%%%%%%%%%%%%%%%%%%%%%%%%%%%%%%%%%

So the final proof should follow these steps, with comments explaining each part.
</think>

```isabelle
theory mathd_algebra_44
  imports Complex_Main
begin

(* Lemma to perform substitution in linear equations *)
lemma solve_linear_substitution:
  fixes a b c d x y :: real
  assumes "x = a - b * y" and "y = c * x + d"
  shows "x = (a - b * (c * x + d))" 
proof -
  from assms(2) have "y = c * x + d" by simp
  from assms(1) have "x = a - b * y" by simp
  then have "x = a - b * (c * x + d)" by (metis assms(2))
  thus ?thesis by simp
qed

(* Formal statement from the input *)
theorem mathd_algebra_44:
  fixes s t :: real
  assumes "s = 9 - 2 * t"
    and "t = 3 * s + 1" 
  shows "s = 1 \<and> t = 4"
proof -
  (* Step 1: Substitute t from the second equation into the first equation. *)
  have "s = 9 - 2 * (3 * s + 1)" 
    using solve_linear_substitution[OF assms(1) assms(2)] by simp

  (* Step 2: Simplify the equation to isolate s. *)
  then have "s = 9 - 6 * s - 2" 
    by (simp add: algebra_simps)

  (* Step 3: Combine like terms to solve for s. *)
  then have "s + 6 * s = 7" 
    by (simp add: add.commute)

  (* Step 4: Simplify to find s = 1. *)
  then have "7 * s = 7" 
    by (simp add: algebra_simps)

  (* Step 5: Solve for s. *)
  then have "s = 1" 
    by (simp add: mult.commute)

  (* Step 6: Substitute s = 1 into the second equation to find t. *)
  with assms(2) have "t = 3 * 1 + 1" 
    by simp

  (* Step 7: Simplify to find t = 4. *)
  then have "t = 4" 
    by simp

  (* Step 8: Conclude the solution. *)
  thus ?thesis 
    by (metis s = 1 t = 4)
qed

end
```
